s/annotate/freshen/g

Abstract_Formula.thy
@@ -14,15 +14,15 @@ lemma fset_fset_from_list[simp]: "fset (fset_from_list l) = set l"  by transfer 
 end
 
 locale Abstract_Formulas =
-  fixes annotate :: "'annot \<Rightarrow> 'preform \<Rightarrow> 'form"
+  fixes freshen :: "'annot \<Rightarrow> 'preform \<Rightarrow> 'form"
   fixes pre_fv :: "'preform \<Rightarrow> 'var set"
   fixes fv :: "'form \<Rightarrow> ('var \<times> 'annot) set"
   fixes subst :: "'subst \<Rightarrow> 'form \<Rightarrow> 'form"
   fixes ran_fv :: "'subst \<Rightarrow> ('var \<times> 'annot) set"
   fixes closed :: "'preform \<Rightarrow> bool"
-  assumes annotate_preserves_fv: "fst ` fv (annotate a pf) = pre_fv pf"
+  assumes annotate_preserves_fv: "fst ` fv (freshen a pf) = pre_fv pf"
   assumes fv_subst: "fv (subst s f) \<subseteq> ran_fv s"
-  assumes closed_eq: "closed pf \<Longrightarrow> subst s1 (annotate a1 pf) = subst s2 (annotate a2 pf)"
+  assumes closed_eq: "closed pf \<Longrightarrow> subst s1 (freshen a1 pf) = subst s2 (freshen a2 pf)"
 
 datatype ('preform, 'var) antecedent =
   Antecedent (a_hyps: "'preform fset") (a_conc: "'preform") (a_fresh: "'var set")
@@ -31,8 +31,8 @@ abbreviation plain_ant :: "'preform \<Rightarrow> ('preform, 'var) antecedent"
   where "plain_ant f \<equiv> Antecedent {||} f {}"
 
 locale Abstract_Rules =
-  Abstract_Formulas annotate pre_fv fv subst
-  for annotate :: "'annot \<Rightarrow> 'preform \<Rightarrow> 'form"
+  Abstract_Formulas freshen pre_fv fv subst
+  for freshen :: "'annot \<Rightarrow> 'preform \<Rightarrow> 'form"
   and pre_fv :: "'preform \<Rightarrow> 'var set"
   and fv :: "'form \<Rightarrow> ('var \<times> 'annot) set"
   and subst :: "'subst \<Rightarrow> 'form \<Rightarrow> 'form" +
@@ -46,10 +46,10 @@ begin
 end
 
 locale Abstract_Task =
-  Abstract_Rules ran_fv closed annotate pre_fv fv subst antecedent consequent rules
+  Abstract_Rules ran_fv closed freshen pre_fv fv subst antecedent consequent rules
   for  ran_fv :: "'subst \<Rightarrow> ('var \<times> 'annot) set" 
     and closed :: "'preform \<Rightarrow> bool" 
-    and annotate :: "'annot \<Rightarrow> 'preform \<Rightarrow> 'form" 
+    and freshen :: "'annot \<Rightarrow> 'preform \<Rightarrow> 'form" 
     and pre_fv :: "'preform \<Rightarrow> 'var set" 
     and fv :: "'form \<Rightarrow> ('var \<times> 'annot) set" 
     and subst :: "'subst \<Rightarrow> 'form \<Rightarrow> 'form" 
@@ -62,17 +62,17 @@ locale Abstract_Task =
   assumes conclusions_closed: "\<forall>c \<in> set conclusions. closed a"
   assumes no_empty_conclusions: "\<forall>xs\<in>sset rules. consequent xs \<noteq> []"
 begin
-  definition ass_forms where "ass_forms = fset_from_list (map (subst undefined) (map (annotate undefined) assumptions))"
-  definition conc_forms where "conc_forms = fset_from_list (map (subst undefined) (map (annotate undefined) conclusions))"
+  definition ass_forms where "ass_forms = fset_from_list (map (subst undefined) (map (freshen undefined) assumptions))"
+  definition conc_forms where "conc_forms = fset_from_list (map (subst undefined) (map (freshen undefined) conclusions))"
 
-  lemma subst_annotate_in_ass_formsI:
+  lemma subst_freshen_in_ass_formsI:
     assumes "pf \<in> set assumptions"
-    shows "subst s (annotate a pf) |\<in>| ass_forms"
+    shows "subst s (freshen a pf) |\<in>| ass_forms"
       using assms ass_forms_def assumptions_closed closed_eq by fastforce
 
-  lemma subst_annotate_in_conc_formsI:
+  lemma subst_freshen_in_conc_formsI:
     assumes "pf \<in> set conclusions"
-    shows "subst s (annotate a pf) |\<in>| conc_forms"
+    shows "subst s (freshen a pf) |\<in>| conc_forms"
       using assms conc_forms_def conclusions_closed closed_eq by fastforce
 end
 
